ArityEtaExpansion: Es fehlen noch Lemmas zu subst bzw. Aexp und Aheap

Launchbury/ArityEtaExpand.thy
@@ -6,11 +6,29 @@ fun lift_transform :: "(Arity \<Rightarrow> exp \<Rightarrow> exp) \<Rightarrow>
   where "lift_transform t Ibottom  e = e"
   |     "lift_transform t (Iup a) e = t a e"
 
+lemma lift_transform_eqvt[eqvt]: "\<pi> \<bullet>  lift_transform t a e = lift_transform (\<pi> \<bullet> t) (\<pi> \<bullet> a) (\<pi> \<bullet> e)"
+  by (cases "(t,a,e)" rule: lift_transform.cases) simp_all
+
 lemma lift_transform_up[simp]: "lift_transform t (up\<cdot>a) e = t a e"
   unfolding up_def by (simp add: cont_Iup)
 
+lemma lift_transform_bot[simp]: "lift_transform t \<bottom> e = e"
+  by (metis inst_up_pcpo lift_transform.simps(1))
+
+lemma lift_transform_fun_cong[fundef_cong]:
+  "(\<And> a. t1 a e1 = t2 a e1) \<Longrightarrow> a1 = a2 \<Longrightarrow> e1 = e2 \<Longrightarrow> lift_transform t1 a1 e1 = lift_transform t2 a2 e2"
+  by (cases "(t2,a2,e2)" rule: lift_transform.cases) auto
+
+lemma subst_lift_transform: 
+  assumes "\<And> a. (t a e)[x ::= y] = t a (e[x ::= y])"
+  shows "(lift_transform t a e)[x ::=y] = lift_transform t a (e[x ::= y])"
+  using assms by (cases a) auto
+
 definition map_transform :: "(Arity \<Rightarrow> exp \<Rightarrow> exp) \<Rightarrow> AEnv \<Rightarrow> heap \<Rightarrow> heap"
   where "map_transform t ae = map_ran (\<lambda> x e . lift_transform t (ae x) e)"
+
+lemma map_transform_eqvt[eqvt]: "\<pi> \<bullet> map_transform t ae = map_transform (\<pi> \<bullet> t) (\<pi> \<bullet> ae)"
+  unfolding map_transform_def by simp
 
 lemma domA_map_transform[simp]: "domA (map_transform t ae \<Gamma>) = domA \<Gamma>"
   unfolding map_transform_def by simp
@@ -18,6 +36,10 @@ lemma domA_map_transform[simp]: "domA (map_transform t ae \<Gamma>) = domA \<Gam
 lemma map_transform_delete:
   "map_transform t ae (delete x \<Gamma>) = delete x (map_transform t ae \<Gamma>)"
   unfolding map_transform_def by (simp add: map_ran_delete)
+
+lemma map_transform_Nil:
+  "map_transform t ae [] = []"
+  unfolding map_transform_def by simp
 
 lemma map_transform_Cons:
   "map_transform t ae ((x,e)# \<Gamma>) = (x, lift_transform t (ae x) e) #  (map_transform t ae \<Gamma>)"
@@ -27,12 +49,37 @@ lemma map_transform_append:
   "map_transform t ae (\<Delta>@\<Gamma>) = map_transform t ae \<Delta> @ map_transform t ae \<Gamma>"
   unfolding map_transform_def by (simp add: map_ran_append)
 
+lemma map_transform_fundef_cong[fundef_cong]:
+  "(\<And>x e a. (x,e) \<in> set m1 \<Longrightarrow> t1 a e = t2 a e) \<Longrightarrow> ae1 = ae2 \<Longrightarrow> m1 = m2 \<Longrightarrow> map_transform t1 ae1 m1 = map_transform t2 ae2 m2"
+  by (induction m2 arbitrary: m1)
+     (fastforce simp add: map_transform_Nil map_transform_Cons intro!: lift_transform_fun_cong)+
+
 lemma map_transform_cong:
   "(\<And>x. x \<in> domA m1 \<Longrightarrow> ae x = ae' x) \<Longrightarrow> m1 = m2 \<Longrightarrow> map_transform t ae m1 = map_transform t ae' m2"
   unfolding map_transform_def by (auto intro!: map_ran_cong dest: domA_from_set)
 
 lemma map_of_map_transform: "map_of (map_transform t ae \<Gamma>) x = map_option (lift_transform t (ae x)) (map_of \<Gamma> x)"
   unfolding map_transform_def by (simp add: map_ran_conv)
+
+lemma supp_map_transform_step:
+  assumes "\<And> x e a. (x, e) \<in> set \<Gamma> \<Longrightarrow> supp (t a e) \<subseteq> supp e"
+  shows "supp (map_transform t ae \<Gamma>) \<subseteq> supp \<Gamma>"
+  using assms
+    apply (induction \<Gamma>)
+    apply (auto simp add: supp_Nil supp_Cons map_transform_Nil map_transform_Cons supp_Pair pure_supp)
+    apply (case_tac "ae a")
+    apply (fastforce)+
+    done
+
+lemma subst_map_transform: 
+  assumes "\<And> x' e a. (x',e) : set \<Gamma> \<Longrightarrow> (t a e)[x ::= y] = t a (e[x ::= y])"
+  shows "(map_transform t ae \<Gamma>)[x ::h=y] = map_transform t ae (\<Gamma>[x ::h= y])"
+  using assms
+  apply (induction \<Gamma>)
+  apply (auto simp add: map_transform_Nil map_transform_Cons)
+  apply (subst subst_lift_transform)
+  apply auto
+  done
 
 locale supp_bounded_transform = 
   fixes trans :: "Arity \<Rightarrow> exp \<Rightarrow> exp"
@@ -52,25 +99,22 @@ begin
     by (auto simp add: fresh_star_def)
 end
 
-locale Has_Aeta_expand_transform = 
-  fixes Aeta_expand_transform :: "Arity \<Rightarrow> exp \<Rightarrow> exp"
-begin
-
-(*
-  fun Aeta_expand_transform' :: "Arity\<^sub>\<bottom> \<Rightarrow> exp \<Rightarrow> exp" 
-  where "Aeta_expand_transform' (Iup a) e = Aeta_expand_transform a e"
-   |    "Aeta_expand_transform' Ibottom e = e"
-
-  lemma [simp]: "Aeta_expand_transform' (up\<cdot>a) e = Aeta_expand_transform a e" unfolding up_def by (simp add: cont_Iup)
-*)
-
-end
-
 
 lift_definition Aeta_expand :: "Arity \<Rightarrow> exp \<Rightarrow> exp"  is "\<lambda> a e. eta_expand a e".
 
+lemma Aeta_expand_eqvt[eqvt]: "\<pi> \<bullet> Aeta_expand a e = Aeta_expand (\<pi> \<bullet> a) (\<pi> \<bullet> e)"
+  apply (cases a)
+  apply simp
+  apply transfer
+  apply simp
+  done
+
 lemma Aeta_expand_0[simp]: "Aeta_expand 0 e = e"
   by transfer simp
+
+lemma subst_Aeta_expand:
+  "(Aeta_expand n e)[x::=y] = Aeta_expand n e[x::=y]"
+  by transfer (rule subst_eta_expand)
 
 lemma Aeta_expand_correct:
   assumes "ae ` upds S \<subseteq> {up \<cdot> 0}"  
@@ -99,8 +143,126 @@ interpretation supp_bounded_transform Aeta_expand
   apply (auto simp add: fresh_def)
   done
 
-locale ArityEtaExpand = CorrectArityAnalysisAheap + Has_Aeta_expand_transform
+locale ArityEtaExpand = CorrectArityAnalysisAheap
 begin
+
+  nominal_function Aeta_expand_transform where
+    "Aeta_expand_transform a (App e x) = App (Aeta_expand_transform (inc\<cdot>a) e) x"
+  | "Aeta_expand_transform a (Lam [x]. e) = Lam [x].(Aeta_expand_transform (pred\<cdot>a) e)"
+  | "Aeta_expand_transform a (Var x) = Var x"
+  | "Aeta_expand_transform a (Terms.Let \<Delta> e) = Terms.Let (map_transform Aeta_expand (Aheap \<Delta>\<cdot>(Aexp e\<cdot>a)) (map_transform Aeta_expand_transform (Aheap \<Delta>\<cdot>(Aexp e\<cdot>a)) \<Delta>)) (Aeta_expand_transform a e)"
+  proof-
+  case goal1
+    thus ?case
+    unfolding eqvt_def Aeta_expand_transform_graph_aux_def
+    apply rule
+    apply perm_simp
+    apply (rule refl)
+    done
+  case (goal3 P x)
+    show ?case
+    proof (cases x)
+      fix a b
+      assume "x = (a, b)"
+      thus ?case
+      using goal3
+      apply (cases b rule:Terms.exp_strong_exhaust)
+      apply auto
+      done
+    qed
+  next
+case (goal8 a x e a' x' e')
+  from goal8(5)
+  have "a' = a" and  "Lam [x]. e = Lam [x']. e'" by simp_all
+  from this(2)
+  show ?case
+  unfolding `a' = a`
+  proof(rule eqvt_lam_case)
+    fix \<pi> :: perm
+
+    assume "supp \<pi> \<sharp>* (Lam [x]. e)" 
+    hence *: "supp \<pi> \<sharp>* Lam [x]. Aeta_expand_transform_sumC (pred\<cdot>a, e)"
+      by (auto simp add: fresh_star_def fresh_def  exp_assn.supp supp_Pair pure_supp exp_assn.fsupp dest!:  set_mp[OF supp_eqvt_at[OF goal8(1)], rotated])
+
+    have "Lam [(\<pi> \<bullet> x)]. Aeta_expand_transform_sumC (pred\<cdot>a, \<pi> \<bullet> e) = \<pi> \<bullet> (Lam [x]. Aeta_expand_transform_sumC (pred\<cdot>a, e))"
+      by (simp add: eqvt_at_apply'[OF goal8(1)])
+    also have "\<dots> = Lam [x]. Aeta_expand_transform_sumC (pred\<cdot>a, e)"
+      by (rule perm_supp_eq[OF *])
+    finally show "Lam [(\<pi> \<bullet> x)]. Aeta_expand_transform_sumC (pred\<cdot>a, \<pi> \<bullet> e) = Lam [x]. Aeta_expand_transform_sumC (pred\<cdot>a, e)" by simp
+  qed
+next
+case (goal13 a as body a' as' body')
+  from supp_eqvt_at[OF goal13(1)]
+  have "\<And> x e a. (x, e) \<in> set as \<Longrightarrow> supp (Aeta_expand_transform_sumC (a, e)) \<subseteq> supp e"
+    by (auto simp add: exp_assn.fsupp supp_Pair pure_supp)
+  hence supp_map: "\<And>ae. supp (map_transform (\<lambda>x0 x1. Aeta_expand_transform_sumC (x0, x1)) ae as) \<subseteq> supp as"
+    by (rule supp_map_transform)    
+
+  from goal13(9)
+  have "a' = a" and  "Terms.Let as body = Terms.Let as' body'" by simp_all
+  from this(2)
+  show ?case
+  unfolding `a' = a`
+  proof (rule eqvt_let_case)
+    fix \<pi> :: perm
+    assume "supp \<pi> \<sharp>* Terms.Let as body"
+    hence *: "supp \<pi> \<sharp>* Terms.Let (map_transform Aeta_expand (Aheap as\<cdot>(Aexp body\<cdot>a)) (map_transform (\<lambda>x0 x1. Aeta_expand_transform_sumC (x0, x1)) (Aheap as\<cdot>(Aexp body\<cdot>a)) as)) (Aeta_expand_transform_sumC (a, body))"
+      by (auto simp add: fresh_star_def fresh_def  Let_supp supp_Pair pure_supp exp_assn.fsupp
+               dest!:  set_mp[OF supp_eqvt_at[OF goal13(2)], rotated] set_mp[OF supp_map_transform] set_mp[OF supp_map])
+
+    have "Terms.Let (map_transform Aeta_expand (Aheap (\<pi> \<bullet> as)\<cdot>(Aexp (\<pi> \<bullet> body)\<cdot>a)) (map_transform (\<lambda>x xa. (\<pi> \<bullet> Aeta_expand_transform_sumC) (x, xa)) (Aheap (\<pi> \<bullet> as)\<cdot>(Aexp (\<pi> \<bullet> body)\<cdot>a)) (\<pi> \<bullet> as))) ((\<pi> \<bullet> Aeta_expand_transform_sumC) (a, \<pi> \<bullet> body)) = 
+        \<pi> \<bullet> (Terms.Let (map_transform Aeta_expand (Aheap as\<cdot>(Aexp body\<cdot>a)) (map_transform (\<lambda>x0 x1. Aeta_expand_transform_sumC (x0, x1)) (Aheap as\<cdot>(Aexp body\<cdot>a)) as)) (Aeta_expand_transform_sumC (a, body)))"
+       by (simp del: Let_eq_iff Pair_eqvt add:  eqvt_at_apply[OF goal13(2)])
+    also have "\<dots> = (Terms.Let (map_transform Aeta_expand (Aheap as\<cdot>(Aexp body\<cdot>a)) (map_transform (\<lambda>x0 x1. Aeta_expand_transform_sumC (x0, x1)) (Aheap as\<cdot>(Aexp body\<cdot>a)) as)) (Aeta_expand_transform_sumC (a, body)))"
+      by (rule perm_supp_eq[OF *])
+    also
+    have "map_transform (\<lambda>x0 x1. Aeta_expand_transform_sumC (x0, x1)) (Aheap (\<pi> \<bullet> as)\<cdot>(Aexp (\<pi> \<bullet> body)\<cdot>a)) (\<pi> \<bullet> as)
+        = map_transform (\<lambda>x xa. (\<pi> \<bullet> Aeta_expand_transform_sumC) (x, xa)) (Aheap (\<pi> \<bullet> as)\<cdot>(Aexp (\<pi> \<bullet> body)\<cdot>a)) (\<pi> \<bullet> as)"
+        apply (rule map_transform_fundef_cong[OF _ refl refl])
+        apply (subst (asm) set_eqvt[symmetric])
+        apply (subst (asm) mem_permute_set)
+        apply (auto simp add: permute_self  dest: eqvt_at_apply''[OF goal13(1)[where aa = "(- \<pi> \<bullet> a)" for a], where p = \<pi>, symmetric])
+        done
+    moreover
+    have " ((\<pi> \<bullet> Aeta_expand_transform_sumC) (a, \<pi> \<bullet> body)) =  (Aeta_expand_transform_sumC) (a, \<pi> \<bullet> body)"
+      using eqvt_at_apply''[OF goal13(2), where p = \<pi>]  by (simp add: permute_pure)
+    ultimately
+    show "Terms.Let (map_transform Aeta_expand (Aheap (\<pi> \<bullet> as)\<cdot>(Aexp (\<pi> \<bullet> body)\<cdot>a)) (map_transform (\<lambda>x0 x1. Aeta_expand_transform_sumC (x0, x1)) (Aheap (\<pi> \<bullet> as)\<cdot>(Aexp (\<pi> \<bullet> body)\<cdot>a)) (\<pi> \<bullet> as))) (Aeta_expand_transform_sumC (a, \<pi> \<bullet> body)) =
+         Terms.Let (map_transform Aeta_expand (Aheap as\<cdot>(Aexp body\<cdot>a)) (map_transform (\<lambda>x0 x1. Aeta_expand_transform_sumC (x0, x1)) (Aheap as\<cdot>(Aexp body\<cdot>a)) as)) (Aeta_expand_transform_sumC (a, body))" by metis
+  qed
+qed auto
+nominal_termination by lexicographic_order
+
+lemma supp_Aeta_expand_transform: "supp (Aeta_expand_transform a e) \<subseteq> supp e"
+  by (induction rule: Aeta_expand_transform.induct)
+     (auto simp add: exp_assn.supp Let_supp dest!: set_mp[OF supp_map_transform] set_mp[OF supp_map_transform_step] )
+
+lemma subst_Aeta_expand_transform: "(Aeta_expand_transform a e)[x ::= y] = Aeta_expand_transform a e[x ::= y]"
+proof (nominal_induct e avoiding: x y arbitrary: a  rule: exp_strong_induct_set)
+  case (Let \<Delta> body x y)
+    moreover
+    have "Aheap \<Delta>[x::h=y] = Aheap \<Delta>" sorry
+    moreover
+    have "(Aexp body[x::=y]\<cdot>a) f|` domA \<Delta> = (Aexp body\<cdot>a) f|` domA \<Delta>"
+      sorry
+    hence "Aheap \<Delta>\<cdot>(Aexp body[x::=y]\<cdot>a) = Aheap \<Delta>\<cdot>(Aexp body\<cdot>a)"
+      sorry
+    ultimately
+    show ?case
+    apply (auto simp add: fresh_star_Pair simp del: Let_eq_iff)
+    apply (rule arg_cong) back
+    apply (subst subst_map_transform)
+    apply (rule subst_Aeta_expand)
+    apply (subst subst_map_transform)
+    apply assumption
+    apply (rule map_transform_cong)
+    apply simp
+    apply (rule map_transform_cong)
+    apply simp
+    apply simp
+    done
+qed auto
+
 
   fun Atransform :: "(AEnv \<times> Arity) \<Rightarrow> conf \<Rightarrow> conf"
   where "Atransform (ae, a) (\<Gamma>, e, S) =
@@ -108,12 +270,6 @@ begin
      Aeta_expand_transform a e,
      S)"
 
-  (*
-  inductive consistent  where
-    [intro!]: "AE_consistent ae (\<Gamma>, e, S) \<Longrightarrow> Astack ae S \<sqsubseteq> a \<Longrightarrow> Aexp e \<cdot> a \<sqsubseteq> ae \<Longrightarrow> consistent (ae, a) (\<Gamma>, e, S)"
-  declare consistent.cases[elim!]
-  *)
-  
   inductive consistent :: "(AEnv \<times> Arity) \<Rightarrow> conf \<Rightarrow> bool" where
     consistentI[intro!]: 
     "edom ae \<subseteq> domA \<Gamma> \<union> upds S
@@ -128,28 +284,12 @@ begin
   inductive_cases consistentE[elim!]: "consistent (ae, a) (\<Gamma>, e, S)"
 
 
-  lemma foobar[simp]:
-    "Aeta_expand_transform a (App e x) = App (Aeta_expand_transform (inc\<cdot>a) e) x"
-    "Aeta_expand_transform a (Lam [x]. e) = Lam [x].(Aeta_expand_transform (pred\<cdot>a) e)"
-    "Aeta_expand_transform a (Var x) = Var x"
-    "Aeta_expand_transform a (Terms.Let \<Delta> e) = Terms.Let (map_transform Aeta_expand (Aheap \<Delta>\<cdot>(Aexp e\<cdot>a)) (map_transform Aeta_expand_transform (Aheap \<Delta>\<cdot>(Aexp e\<cdot>a)) \<Gamma>)) (Aeta_expand_transform a e)"
-    "Aeta_expand_transform a (e[x ::= z]) = (Aeta_expand_transform a e)[x ::= z]"
-    "at \<sharp> Aeta_expand_transform a e \<longleftrightarrow> at \<sharp> e"
-    sorry
-
   interpretation supp_bounded_transform Aeta_expand_transform
-    apply default
-    using foobar(6)
-    apply (auto simp add: fresh_def)
-    done
+    by default (auto simp add: fresh_def supp_Aeta_expand_transform)
   
   lemma isLam_Aeta_expand_transform[simp]:
     "isLam (Aeta_expand_transform a e) \<longleftrightarrow> isLam e"
-    apply (induction e rule:isLam.induct)
-    apply (auto simp add: foobar(4)[where a = a])
-    apply (subst (asm) foobar) (* WTF *)
-    apply simp
-    done
+    by (induction e rule:isLam.induct) auto
 
   sublocale AbstractConforms step consistent.
 
@@ -176,19 +316,11 @@ case (app\<^sub>2 \<Gamma> y e x S)
     apply  (auto intro!:  below_trans[OF monofun_cfun_fun[OF Aexp_subst_App_Lam]] simp add: Aexp_App join_below_iff monofun_cfun_arg)
     by (metis image_eqI singletonD subsetCE)
   moreover
-  have "Atransform (ae, a) (\<Gamma>, Lam [y]. e, Arg x # S) \<Rightarrow> Atransform (ae, pred \<cdot> a) (\<Gamma>, e[y::=x], S)" by simp rule
+  have "Atransform (ae, a) (\<Gamma>, Lam [y]. e, Arg x # S) \<Rightarrow> Atransform (ae, pred \<cdot> a) (\<Gamma>, e[y::=x], S)" by (simp add: subst_Aeta_expand_transform[symmetric]) rule
   ultimately
   show ?case by (blast del: consistentI consistentE)
 next
 case (var\<^sub>1 \<Gamma> x e S)
-  (*
-  from var\<^sub>1 have "Aexp (Var x)\<cdot>a \<sqsubseteq> ae" by auto
-  from below_trans[OF Aexp_Var fun_belowD[OF this] ]
-  have "up\<cdot>a \<sqsubseteq> ae x".
-  then obtain u where "ae x = up\<cdot>u" and "a \<sqsubseteq> u" by (cases "ae x") auto
-  moreover
-  hence "x \<in> edom ae" unfolding edom_def by auto
-  *)
   have "consistent (ae, 0) (delete x \<Gamma>, e, Upd x # S)" using var\<^sub>1 by (fastforce  simp add: join_below_iff)
   moreover
   {
@@ -370,7 +502,6 @@ next
     ultimately
     have "Atransform (ae, a) (\<Gamma>, Terms.Let \<Delta> e, S) \<Rightarrow> Atransform (?ae \<squnion> ae, a) (\<Delta> @ \<Gamma>, e, S)"
       apply (simp add: map_transform_append)
-      apply (subst foobar(4))
       apply rule
       using let\<^sub>1(1,2)
       by auto
