Launchbury/ArityAnalysisImpl.thy
@@ -82,7 +82,7 @@ case (goal13 as body as' body')
   qed
 qed auto
 
-nominal_termination by lexicographic_order
+nominal_termination (eqvt) by lexicographic_order
 
 interpretation ArityAnalysis Aexp.
 
@@ -172,6 +172,8 @@ qed
 
 interpretation CorrectArityAnalysis Aexp
 proof default
+  fix \<pi> show "\<pi> \<bullet> Aexp = Aexp" by perm_simp rule
+next
   fix e' y x
   show "Aexp e'[y::=x] \<sqsubseteq> Aexp (App (Lam [y]. e') x)"
     apply (rule cfun_belowI)
@@ -184,8 +186,64 @@ qed simp_all
 definition Aheap where
   "Aheap \<Gamma> = (\<Lambda> ae. (Afix \<Gamma> \<cdot> (ae \<squnion> thunks \<Gamma>) f|` domA \<Gamma>))"
 
+lemma Aheap_eqvt'[eqvt]:
+  "\<pi> \<bullet> (Aheap \<Gamma>) = Aheap (\<pi> \<bullet> \<Gamma>)"
+  unfolding Aheap_def
+  apply perm_simp
+  apply (subst Abs_cfun_eqvt)
+  apply simp
+  apply rule
+  done
+
+(*   moreover
+    have "Aheap \<Delta>[x::h=y] = Aheap \<Delta>" sorry
+    moreover
+    have "(Aexp body[x::=y]\<cdot>a) f|` domA \<Delta> = (Aexp body\<cdot>a) f|` domA \<Delta>"
+      sorry
+    hence "Aheap \<Delta>\<cdot>(Aexp body[x::=y]\<cdot>a) = Aheap \<Delta>\<cdot>(Aexp body\<cdot>a)"
+*)
+
+(*
+lemma foobar:
+  assumes "x \<notin> S" and "y \<notin> S"
+  shows "(Aexp e[x::=y]\<cdot>a) f|` S = (Aexp e\<cdot>a) f|` S"
+using assms
+proof (nominal_induct e avoiding: x y  arbitrary: a  S rule: exp_strong_induct)
+  case (Var v) 
+  thus ?case by auto
+next
+  case (App e v)
+  thus ?case by (auto simp add: env_restr_join simp del: fun_meet_simp)
+next
+  case (Lam v e)
+  thus ?case by (auto simp add: env_restr_join env_delete_restr simp del: fun_meet_simp)
+next
+  case (Let \<Gamma> e)
+  hence "x \<notin> domA \<Gamma> " and "y \<notin> domA \<Gamma>"
+    by (metis (erased, hide_lams) bn_subst domA_not_fresh fresh_def fresh_star_at_base fresh_star_def obtain_fresh subst_is_fresh(2))+
+  
+  note this[simp] Let(1,2)[simp]
+
+  from Let
+  show ?case apply (auto simp add: fresh_star_Pair)
+
+  have "Aexp (Terms.Let \<Gamma> e)[y::=x]\<cdot>n \<sqsubseteq> Afix \<Gamma>[y::h=x]\<cdot>(Aexp e[y::=x]\<cdot>n \<squnion> thunks \<Gamma>[y::h=x]) f|` ( - domA \<Gamma>)" by (simp add: fresh_star_Pair)
+  also have "(Aexp e[y::=x]\<cdot>n) \<sqsubseteq> (Aexp e\<cdot>n)(y := \<bottom>, x := up\<cdot>0)" by fact
+  also have "thunks \<Gamma>[y::h=x] \<sqsubseteq> (thunks \<Gamma>)(y := \<bottom>, x := up\<cdot>0)" by (rule thunks_subst_approx[OF `y \<notin> domA \<Gamma>`])
+  also have "(Aexp e\<cdot>n)(y := \<bottom>, x := up\<cdot>0) \<squnion> (thunks \<Gamma>)(y := \<bottom>, x := up\<cdot>0) = (Aexp e\<cdot>n \<squnion> thunks \<Gamma>)(y := \<bottom>, x := up\<cdot>0)" by simp
+  also have "Afix \<Gamma>[y::h=x]\<cdot>((Aexp e\<cdot>n \<squnion> thunks \<Gamma>)(y := \<bottom>, x := up\<cdot>0)) \<sqsubseteq> (Afix \<Gamma>\<cdot>(Aexp e\<cdot>n \<squnion> thunks \<Gamma>))(y := \<bottom>, x := up\<cdot>0)"
+    by (rule Afix_subst_approx[OF Let(3) `x \<notin> domA \<Gamma>` `y \<notin> domA \<Gamma>`])
+  also have "(Afix \<Gamma>\<cdot>(Aexp e\<cdot>n \<squnion> thunks \<Gamma>))(y := \<bottom>, x := up\<cdot>0) f|` (- domA \<Gamma>) = (Afix \<Gamma>\<cdot>(Aexp e\<cdot>n \<squnion> thunks \<Gamma>) f|` (- domA \<Gamma>)) (y := \<bottom>, x := up\<cdot>0)" by auto
+  also have "(Afix \<Gamma>\<cdot>(Aexp e\<cdot>n \<squnion> thunks \<Gamma>) f|` (- domA \<Gamma>)) = Aexp (Terms.Let \<Gamma> e)\<cdot>n" by simp
+  finally show ?case by this simp_all
+qed
+*)
+
+
 interpretation CorrectArityAnalysisAheap Aexp Aheap
 proof default
+  fix \<pi> show "\<pi> \<bullet> Aheap = Aheap" by perm_simp rule
+next
   fix \<Gamma> ae
   show "edom (Aheap \<Gamma>\<cdot>ae) \<subseteq> domA \<Gamma>"  unfolding Aheap_def by simp
 
